Yen.thy
@@ -1,0 +1,48 @@
+theory Yen imports CoinClass begin
+
+
+
+datatype Yen = One | Five | Ten | Fifty | Hundred | FiveHundreds
+
+
+instantiation Yen :: coins begin
+fun Yen_unit :: "Yen \<Rightarrow> val" where
+  "Yen_unit One = 1" |
+  "Yen_unit Five = 5" |
+  "Yen_unit Ten = 10" |
+  "Yen_unit Fifty = 50" |
+  "Yen_unit Hundred = 100" |
+  "Yen_unit FiveHundreds = 500"
+
+
+definition val_unit_Yen: "val_unit_Yen \<equiv> Yen_unit"
+
+
+lemma inj_val_unit_Yen: "inj Yen_unit"
+  apply(unfold inj_def)
+  apply(intro allI)
+  apply(rule_tac y=x in Yen.exhaust; auto)
+  apply(rule_tac y=y in Yen.exhaust; auto)
+  apply(rule_tac y=y in Yen.exhaust; auto)
+  apply(rule_tac y=y in Yen.exhaust; auto)
+  apply(rule_tac y=y in Yen.exhaust; auto)
+  apply(rule_tac y=y in Yen.exhaust; auto)
+  apply(rule_tac y=y in Yen.exhaust; auto)
+  done
+
+
+lemma dvd_val_units_Yen: "\<forall>c1 c2. Yen_unit c1 < Yen_unit c2 \<longrightarrow> Yen_unit c1 dvd Yen_unit c2"
+  apply(intro allI)
+  apply(rule_tac y=c1 in Yen.exhaust; auto)
+  apply(rule_tac y=c2 in Yen.exhaust; auto)
+  apply(rule_tac y=c2 in Yen.exhaust; auto)
+  apply(rule_tac y=c2 in Yen.exhaust; auto)
+  apply(rule_tac y=c2 in Yen.exhaust; auto)
+  apply(rule_tac y=c2 in Yen.exhaust; auto)
+  done
+
+
+instance
+  by standard (auto simp add: val_unit_Yen inj_val_unit_Yen dvd_val_units_Yen)
+end
+end
